Proof of contains and findPred specs for skip list

skip_list/inv/lazy_inv.v
@@ -15,26 +15,18 @@ Class gset_list_unionGS Σ := GsetGS {
 }.
 
 Local Open Scope Z.
-Module SkipListInv (Params: SKIP_LIST_PARAMS).
+Module LazyListInv (Params: SKIP_LIST_PARAMS).
   Import Params.
   Module NodeLt := NodeLt Params.
   Export NodeLt.
 
-  Record lazy_gname := mk_lazy_gname {
-    s_auth: gname;
-    s_frac: gname;
-    s_tok: gname
-  }.
-
   Section Proofs.
     Context `{!heapGS Σ, !gset_list_unionGS Σ, lockG Σ} (N : namespace).
-
-    Definition levelN (lvl: Z) := nroot .@ "level" .@ lvl.
 
     Definition node_inv (l: loc) : iProp Σ := 
       ∃ (succ: node_rep), l ↦{#1 / 2} rep_to_node succ.
 
-    Fixpoint list_equiv (L: list node_rep) : iProp Σ :=
+    Fixpoint list_equiv (L: list node_rep) (P: node_rep → iProp Σ) : iProp Σ :=
       match L with
       | nil => True
       | pred :: succs => 
@@ -53,80 +45,36 @@ Module SkipListInv (Params: SKIP_LIST_PARAMS).
                        ∗
                        is_lock γ (node_lock pred) (node_inv l)
                        ∗
-                       list_equiv succs
+                       P succ
+                       ∗
+                       list_equiv succs P
         end
       end.
 
-    Definition lazy_list_inv (head: node_rep) (S: gset node_rep) : iProp Σ := 
+    Definition lazy_list_inv (head: node_rep) (S: gset node_rep) (P: node_rep → iProp Σ) : iProp Σ :=
       ∃ (L: list node_rep),
       ⌜ Permutation L (elements S) ⌝
       ∗
       ⌜ Sorted node_lt ([head] ++ L ++ [tail]) ⌝
       ∗
-      list_equiv ([head] ++ L)
-    .
-
-    Fixpoint skip_list_equiv (head: node_rep) (lvl: Z) (L: list (list node_rep)) (S St: gset node_rep) : iProp Σ :=
-      match L with
-      | nil => True
-      | top :: bots =>
-        match bots with
-        | nil => ⌜ St = S ⌝
-                 ∗
-                 inv (levelN lvl) (lazy_list_inv head St)
-                 ∗
-                 ⌜ node_down head = None ⌝
-                 ∗
-                 ⌜ lvl = 0 ⌝
-                 
-        | _ :: _ => ∃ (Sb: gset node_rep) (l: loc) (down: node_rep),
-                    ⌜ St ⊆ Sb ⊆ S ⌝
-                    ∗
-                    inv (levelN lvl) (lazy_list_inv head St)
-                    ∗
-                    ⌜ node_down head = Some l ⌝
-                    ∗
-                    l ↦ rep_to_node down
-                    ∗
-                    skip_list_equiv down (lvl - 1) bots S Sb
-        end
-      end.
-
-    Definition skip_list_inv (head: node_rep) (S: gset node_rep) : iProp Σ := 
-      ∃ (St: gset node_rep) (L: list (list node_rep)),
-      ⌜ St ⊆ S ⌝
-      ∗
-      skip_list_equiv head MAX_HEIGHT L S St
-    .
-
-    Definition is_skip_list (v: val) (Skeys: gset Z) : iProp Σ := 
-      ∃ (l:loc) (head: node_rep) (S: gset node_rep),
-      ⌜ key_equiv S Skeys ⌝
-      ∗
-      ⌜ #l = v ⌝
-      ∗
-      l ↦ rep_to_node head
-      ∗
-      ⌜ node_key head = INT_MIN ⌝
-      ∗
-      inv N (skip_list_inv head S).
+      list_equiv ([head] ++ L) P.
     
 
-    Lemma list_equiv_cons (rep: node_rep) (L: list node_rep) :
-      list_equiv (rep :: L)
-        ⊢ (list_equiv L ∗ (list_equiv L -∗ list_equiv (rep :: L)))
+    Lemma list_equiv_cons (rep: node_rep) (L: list node_rep) (P: node_rep → iProp Σ) :
+      list_equiv (rep :: L) P ⊢ 
+        (list_equiv L P ∗ (list_equiv L P -∗ list_equiv (rep :: L) P))
     .
     Proof.
       destruct L as [|n].
       * iIntros "Hrep". by iFrame.
-      * iIntros "Hlist". iDestruct "Hlist" as (l γ) "(Hsome & Hpt & Hlock & Hmatch)".
+      * iIntros "Hlist". iDestruct "Hlist" as (l γ) "(Hsome & Hpt & Hlock & HP & Hmatch)".
         iFrame. iIntros "Hlist". iFrame.
         iExists l, γ. iFrame.
     Qed.
 
-    Lemma list_equiv_split (pred succ: node_rep) (L L1 L2: list node_rep) :
+    Lemma list_equiv_split (pred succ: node_rep) (L L1 L2: list node_rep) (P: node_rep → iProp Σ) :
       L ++ [tail] = L1 ++ [pred; succ] ++ L2 →
-      list_equiv L ⊢ 
+      list_equiv L P ⊢ 
         ∃ (l: loc) (γ: gname),
           ⌜ node_next pred = Some l ⌝
           ∗
@@ -134,7 +82,7 @@ Module SkipListInv (Params: SKIP_LIST_PARAMS).
           ∗
           is_lock γ (node_lock pred) (node_inv l)
           ∗
-          (l ↦{#1 / 2} (rep_to_node succ) -∗ list_equiv L)
+          (l ↦{#1 / 2} (rep_to_node succ) -∗ list_equiv L P)
     .
     Proof.
       revert L. induction L1 => L HL.
@@ -145,15 +93,15 @@ Module SkipListInv (Params: SKIP_LIST_PARAMS).
         - inversion HL'; subst.
           iIntros "Hlist". 
           iDestruct "Hlist" as (l γ) "(#Hsome & Hpt & #Hlock)".
-          iExists l, γ. iFrame "#"; iFrame.
+          iExists l, γ. iFrame "# ∗".
           iIntros "Hpt". 
-          iExists l, γ. iFrame "#"; iFrame.
+          iExists l, γ. iFrame "# ∗".
         - inversion HL'; subst.
           iIntros "Hlist". 
           iDestruct "Hlist" as (l γ) "(#Hsome & Hpt & #Hlock & Hmatch)".
-          iExists l, γ. iFrame "#"; iFrame.
+          iExists l, γ. iFrame "# ∗".
           iIntros "Hpt". 
-          iExists l, γ. iFrame "#"; iFrame.
+          iExists l, γ. iFrame "# ∗".
       + destruct L as [|curr L].
         { 
           exfalso. inversion HL  as [[H0 HL']]; subst. 
@@ -176,9 +124,9 @@ Module SkipListInv (Params: SKIP_LIST_PARAMS).
         iApply "Himp". iApply "Himp'". iFrame.
     Qed.
 
-    Lemma list_equiv_invert (L: list node_rep) (head pred: node_rep) :
-      pred = head ∨ In pred L →
-      list_equiv ([head] ++ L) ⊢ 
+    Lemma list_equiv_invert_L (L: list node_rep) (head pred: node_rep) (P: node_rep → iProp Σ) :
+      In pred L →
+      list_equiv ([head] ++ L) P ⊢ 
         ∃ (succ: node_rep) (l: loc) (γ: gname), 
           (⌜ In succ L ⌝ ∨ ⌜ succ = tail ⌝)
           ∗
@@ -188,65 +136,92 @@ Module SkipListInv (Params: SKIP_LIST_PARAMS).
           ∗ 
           is_lock γ (node_lock pred) (node_inv l)
           ∗
-          (l ↦{#1/2} (rep_to_node succ) -∗ list_equiv ([head] ++ L)).
+          P pred
+          ∗
+          (l ↦{#1/2} (rep_to_node succ) ∗ P pred -∗ list_equiv ([head] ++ L) P).
     Proof.
-      intros Hin; inversion Hin as [|Hin_L]; subst.
-      + iIntros "Hlist". destruct L as [|succ' L].
-        - iDestruct "Hlist" as (l γ) "(%Hsome & Hpt & #Hlock)".
-          iExists tail, l, γ. iFrame; iFrame "#".
+      intros Hin.
+      iIntros "Hlist".
+
+      iRevert (head Hin) "Hlist".
+      iInduction L as [|succ L] "IHL"; iIntros (head) "Hin"; first by iExFalso.
+      iDestruct "Hin" as "[%Heq|Hin]"; subst; iIntros "Hlist".
+      + iDestruct "Hlist" as (l γ) "(%Hsome & Hpt & #Hlock & HP & Hlist)".
+        destruct L as [|succ' L]; subst.
+        - iDestruct "Hlist" as (l' γ') "(%Hsome' & Hpt' & #Hlock')".
+          iExists tail, l', γ'. iFrame "# ∗".
           iSplit; first by iRight. iSplit; first done.
-          iIntros "Hpt". iExists l, γ.
-          by iFrame; iFrame "#".
-        - iDestruct "Hlist" as (l γ) "(%Hsome & Hpt & #Hlock & ?)".
-          iExists succ', l, γ. iFrame; iFrame "#".
-          iSplit; first by repeat iLeft. iSplit; first done. 
-          iIntros "Hpt". iExists l, γ.
-          by iFrame; iFrame "#".
-      + simpl in Hin_L; clear Hin.
-        iIntros "Hlist".
-        iPoseProof (list_equiv_cons with "Hlist") as "(Hlist & Himp)".
-        iRevert (head Hin_L) "Hlist Himp".
-        iInduction L as [|succ' L] "IHL"; iIntros (head) "Hin"; first by iExFalso.
-        iDestruct "Hin" as "[%Heq|Hin]"; subst; iIntros "Hlist Himp".
-        - destruct L as [|succ'' L]; subst.
-          * iDestruct "Hlist" as (l γ) "(%Hsome & Hpt & #Hlock)".
-            iExists tail, l, γ. iFrame; iFrame "#".
-            iSplit; first by iRight. iSplit; first done.
-            iIntros "Hpt". iApply "Himp". iExists l, γ. 
-            by iFrame; iFrame "#".
-          * iDestruct "Hlist" as (l γ) "(%Hsome & Hpt & #Hlock & Hmatch)".
-            iExists succ'', l, γ. 
-            iSplit; first by iLeft; iRight; iLeft. iSplit; first done.
-            iFrame "Hpt"; iFrame "Hlock".
-            iIntros "Hpt". iApply "Himp".
-            iExists l, γ. by iFrame; iFrame "#".
-        - iPoseProof (list_equiv_cons with "Hlist") as "(Hlist & Himp')".
-          iPoseProof ("IHL" with "Hin") as "Himp''".
-          iPoseProof ("Himp''" with "Hlist") as "Himp''".
-          iPoseProof ("Himp''" with "Himp'") as "Hlist".
-          iDestruct "Hlist" as (succ l γ) "(Hsucc & Hsome & Hpt & Hlock & Himp')".
-          iExists succ, l, γ. iFrame; iFrame "#".
-          iSplit.
-          {
-            iDestruct "Hsucc" as "[Hin|Heq]".
-            by iLeft; iRight. by iRight.
-          }
-          iIntros "Hpt".
-          iApply "Himp". by iApply "Himp'".
+          iIntros "(Hpt' & HP)". 
+          iExists l, γ. iFrame "# ∗". iSplit; first done.
+          iExists l', γ'. by iFrame "# ∗".
+        - iDestruct "Hlist" as (l' γ') "(%Hsome' & Hpt' & #Hlock' & Hmatch)".
+          iExists succ', l', γ'. iFrame "# ∗".
+          iSplit; first by iLeft; iRight; iLeft. iSplit; first done.
+          iIntros "(Hpt' & HP)". 
+          iExists l, γ. iFrame "# ∗". iSplit; first done.
+          iExists l', γ'. by iFrame "# ∗".
+      + iPoseProof (list_equiv_cons with "Hlist") as "(Hlist & Himp)".
+        iPoseProof ("IHL" with "Hin") as "Himp'".
+        iPoseProof ("Himp'" with "Hlist") as "Hlist".
+        iDestruct "Hlist" as (succ' l γ) "(Hsucc & Hsome & Hpt & Hlock & HP & Himp')".
+        iExists succ', l, γ. iFrame "# ∗".
+        iSplit.
+        {
+          iDestruct "Hsucc" as "[Hin|Heq]".
+          by iLeft; iRight. by iRight.
+        }
+        iIntros "(Hpt' & HP)". 
+        iApply "Himp". iApply "Himp'". iFrame.
     Qed.
 
-    Lemma list_equiv_insert (head pred new succ: node_rep)
-      (L: list node_rep) (l l': loc) (γ': gname) :
+    Lemma list_equiv_invert (L: list node_rep) (head pred: node_rep) (P: node_rep → iProp Σ) :
+      pred = head ∨ In pred L →
+      list_equiv ([head] ++ L) P ⊢ 
+        ∃ (succ: node_rep) (l: loc) (γ: gname), 
+          (⌜ In succ L ⌝ ∨ ⌜ succ = tail ⌝)
+          ∗
+          ⌜ node_next pred = Some l ⌝
+          ∗
+          l ↦{#1/2} (rep_to_node succ)
+          ∗ 
+          is_lock γ (node_lock pred) (node_inv l)
+          ∗
+          (l ↦{#1/2} (rep_to_node succ) -∗ list_equiv ([head] ++ L) P).
+    Proof.
+      intros Hin; destruct Hin as [Heq|Hin]; first subst.
+      + iIntros "Hlist". destruct L as [|succ' L].
+        - iDestruct "Hlist" as (l γ) "(%Hsome & Hpt & #Hlock)".
+          iExists tail, l, γ. iFrame "# ∗".
+          iSplit; first by iRight. iSplit; first done.
+          iIntros "Hpt". iExists l, γ.
+          by iFrame "# ∗".
+        - iDestruct "Hlist" as (l γ) "(%Hsome & Hpt & #Hlock & ?)".
+          iExists succ', l, γ. iFrame "# ∗".
+          iSplit; first by repeat iLeft. iSplit; first done. 
+          iIntros "Hpt". iExists l, γ.
+          by iFrame "# ∗".
+      + iIntros "Hlist".
+        iPoseProof (list_equiv_invert_L with "Hlist") as "Hlist"; first done.
+        iDestruct "Hlist" as (succ l γ) "(? & ? & ? & ? & ? & Himp)".
+        iExists succ, l, γ. iFrame.
+        iIntros "?". iApply "Himp". iFrame.
+    Qed.
+
+    Lemma list_equiv_insert (head pred new succ: node_rep) (L: list node_rep) 
+      (l l': loc) (γ': gname) (P: node_rep → iProp Σ) :
       node_key new < node_key tail →
       node_key pred < node_key new < node_key succ →
       Sorted node_lt ([head] ++ L ++ [tail]) →
       pred = head ∨ In pred L →
-      list_equiv ([head] ++ L) ⊢ 
+      list_equiv ([head] ++ L) P ⊢ 
         ⌜ node_next pred = Some l ⌝ ∗ l↦{#1/2} rep_to_node succ 
         ∗ 
         ⌜ node_next new = Some l' ⌝ ∗ l'↦{#1/2} rep_to_node succ
         ∗
-        is_lock γ' (node_lock new) (node_inv l') -∗ 
+        is_lock γ' (node_lock new) (node_inv l')
+        ∗
+        P new
+        -∗ 
           ∃ (L': list node_rep), 
             l ↦ rep_to_node succ 
             ∗
@@ -254,13 +229,13 @@ Module SkipListInv (Params: SKIP_LIST_PARAMS).
             ∗
             ⌜ Permutation ([head] ++ L') ([head; new] ++ L) ⌝ 
             ∗
-            (l ↦{#1/2} (rep_to_node new) -∗ list_equiv ([head] ++ L')).
+            (l ↦{#1/2} (rep_to_node new) -∗ list_equiv ([head] ++ L') P).
     Proof.
-      iIntros (Hnew Hrange Hsort Hin) "Hlist (Hsome & Hpt & Hsome' & Hpt' & Hlock')".
+      iIntros (Hnew Hrange Hsort Hin) "Hlist (Hsome & Hpt & Hsome' & Hpt' & Hlock' & HP')".
       remember ([head] ++ L) as L' eqn:HeqL'.
       rewrite -in_inv in Hin.
 
-      iRevert (head L HeqL' Hsort Hin) "Hlist Hsome Hpt Hsome' Hpt' Hlock'".
+      iRevert (head L HeqL' Hsort Hin) "Hlist Hsome Hpt Hsome' Hpt' Hlock' HP'".
       iInduction L' as [|pred'] "IHL'".
       { iIntros (head L Hfalse); inversion Hfalse. }
 
@@ -268,7 +243,7 @@ Module SkipListInv (Params: SKIP_LIST_PARAMS).
       inversion HeqL'; subst.
       iIntros (Hin); inversion Hin.
       * subst.
-        iIntros "Hlist %Hsome Hpt %Hsome' Hpt' #Hlock'".
+        iIntros "Hlist %Hsome Hpt %Hsome' Hpt' #Hlock' HP'".
         iExists (new :: L).
         destruct L as [|].
         ** simpl.
@@ -285,7 +260,7 @@ Module SkipListInv (Params: SKIP_LIST_PARAMS).
            iIntros "Hpt". iExists _, _.
            iFrame "# ∗". iSplit; first done.
            iExists _, _. by iFrame "# ∗".
-        ** iDestruct "Hlist" as (l'' γ) "(%Hsome'' & Hpt'' & #Hlock & Hmatch)".
+        ** iDestruct "Hlist" as (l'' γ) "(%Hsome'' & Hpt'' & #Hlock & HP & Hmatch)".
            assert (l = l'') as <- by congruence.
            iDestruct (mapsto_agree with "Hpt Hpt''") as %Heq.
            apply rep_to_node_inj in Heq; subst.
@@ -302,11 +277,11 @@ Module SkipListInv (Params: SKIP_LIST_PARAMS).
            iFrame "# ∗". iSplit; first done.
            iExists _, _. by iFrame "# ∗".
       * destruct L as [|head' L]; first by inversion H0.
-        iIntros "Hlist %Hsome Hpt %Hsome' Hpt' #Hlock'".
+        iIntros "Hlist %Hsome Hpt %Hsome' Hpt' #Hlock' HP'".
 
         simpl in Hsort; apply Sorted_inv in Hsort as (Hsort&Hhd).
-        iDestruct "Hlist" as (l'' γ) "(Hsome'' & Hpt'' & Hlock & Hmatch)".
-        iPoseProof ("IHL'" $! head' L with "[%] [%] [%] [$] [%] [$] [%] [$] [$]") 
+        iDestruct "Hlist" as (l'' γ) "(Hsome'' & Hpt'' & Hlock & HP & Hmatch)".
+        iPoseProof ("IHL'" $! head' L with "[%] [%] [%] [$] [%] [$] [%] [$] [$] [$]") 
           as "Hclose"; auto.
         
         iDestruct "Hclose" as (L') "(Hpt' & %Hsort' & %Hperm' & Himp')".
@@ -330,4 +305,4 @@ Module SkipListInv (Params: SKIP_LIST_PARAMS).
     Qed.
 
   End Proofs.
-End SkipListInv.
+End LazyListInv.
