skip_list/inv/skip_inv.v
@@ -1,0 +1,93 @@
+From Coq Require Import Sorting.Sorted.
+
+From iris.base_logic.lib Require Import invariants.
+From iris.algebra Require Import auth frac_auth gset.
+From iris.heap_lang Require Import proofmode.
+From iris.bi Require Import updates.
+
+From SkipList.lib Require Import lock misc.
+From SkipList.skip_list Require Import node_lt node_rep code key_equiv.
+From SkipList.skip_list.inv Require Import lazy_inv.
+
+
+Local Open Scope Z.
+Module SkipListInv (Params: SKIP_LIST_PARAMS).
+  Import Params.
+  Module Invariant := LazyListInv Params.
+  Export Invariant.
+
+  Section Proofs.
+    Context `{!heapGS Σ, !gset_list_unionGS Σ, lockG Σ} (N : namespace).
+
+    Definition levelN (lvl: Z) := nroot .@ "level" .@ lvl.
+
+    Definition from_sub_list (bot: gset node_rep) (curr: node_rep) : iProp Σ := 
+      ∃ (l: loc) (down: node_rep),
+      ⌜ node_down curr = Some l ⌝
+      ∗
+      l ↦ rep_to_node down
+      ∗
+      ⌜ down ∈ bot ⌝
+      ∗
+      ⌜ node_key curr = node_key down ⌝.
+
+    Definition from_bot_list (curr: node_rep) : iProp Σ := 
+      ⌜ node_down curr = None ⌝.
+
+    Fixpoint skip_list_equiv (head: node_rep) (lvl: Z) (L: list (gset node_rep)) (S: gset node_rep) : iProp Σ :=
+      match L with
+      | nil => True
+      | top :: bots =>
+        match bots with
+        | nil => inv (levelN lvl) (lazy_list_inv head top from_bot_list)
+                 ∗
+                 ⌜ node_down head = None ⌝
+                 ∗
+                 ⌜ top = S ⌝
+                 
+        | bot :: _ => ∃ (l: loc) (down: node_rep),
+                      inv (levelN lvl) (lazy_list_inv head top (from_sub_list bot))
+                      ∗
+                      ⌜ node_down head = Some l ⌝
+                      ∗
+                      l ↦ rep_to_node down
+                      ∗
+                      ⌜ node_key head = node_key down ⌝
+                      ∗
+                      skip_list_equiv down (lvl - 1) bots S
+        end
+      end.
+
+    Definition is_skip_list (v: val) (Skeys: gset Z) : iProp Σ := 
+      ∃ (l:loc) (head: node_rep) (S: gset node_rep) (L: list (gset node_rep)),
+      ⌜ key_equiv S Skeys ⌝
+      ∗
+      ⌜ #l = v ⌝
+      ∗
+      l ↦ rep_to_node head
+      ∗
+      ⌜ node_key head = INT_MIN ⌝
+      ∗
+      skip_list_equiv head MAX_HEIGHT (∅ :: L) S.
+
+
+    Lemma skip_list_equiv_cons_inv (top_head: node_rep) (lvl: Z) (S: gset node_rep)
+      (L: list (gset node_rep)) (top: gset node_rep) :
+      skip_list_equiv top_head lvl (top :: L) S ⊢ 
+        ∃ (P: node_rep → iProp Σ),
+        inv (levelN lvl) (lazy_list_inv top_head top P)
+        ∗
+        skip_list_equiv top_head lvl (top :: L) S
+    .
+    Proof.
+      destruct L as [|bot].
+      + iIntros "Htop". iExists from_bot_list.
+        iDestruct "Htop" as "(#Hinv & %Hsome & %Hlvl)".
+        by iFrame "#".
+      + iIntros "Hlist". iExists (from_sub_list bot).
+        iDestruct "Hlist" as (l down) "(#Hinv & %Hsome & Hpt & Hmatch)".
+        iFrame "#". iExists l, down. by iFrame.
+    Qed.
+
+  End Proofs.
+End SkipListInv.
