skip_list/spec/contains.v
@@ -4,7 +4,7 @@ From iris.algebra Require Import auth frac_auth gset.
 From iris.heap_lang Require Import proofmode.
 
 From SkipList.lib Require Import lock misc.
-From SkipList.skip_list Require Import inv node_rep code key_equiv.
+From SkipList.skip_list Require Import node_rep code key_equiv.
 From SkipList.skip_list.spec Require Import find.
 
 
@@ -17,50 +17,136 @@ Module ContainsSpec (Params: SKIP_LIST_PARAMS).
   Section Proofs.
     Context `{!heapGS Σ, !gset_list_unionGS Σ, lockG Σ} (N : namespace).
     
-    Theorem findPred_spec (head curr: node_rep) (key: Z) (S: gset node_rep) :
+    Theorem findPred_spec (curr top_head: node_rep) (top: gset node_rep) 
+      (lvl: Z) (key: Z) (L: list (gset node_rep)) (S: gset node_rep) :
       {{{ 
-        inv N (skip_list_inv head S)
+        skip_list_equiv top_head lvl (top :: L) S
         ∗
-        ⌜ curr = head ∨ curr ∈ S ⌝
+        ⌜ curr = top_head ∨ curr ∈ top ⌝
         ∗
         ⌜ node_key curr < key < INT_MAX ⌝
       }}}
         findPred (rep_to_node curr) #key
       {{{ pred succ, RET SOMEV ((rep_to_node pred), (rep_to_node succ));
+        skip_list_equiv top_head lvl (top :: L) S
+        ∗
         ⌜ key ∈ map node_key (elements S) ↔ node_key succ = key ⌝
       }}}.
     Proof.
-    Admitted.
+      iIntros (Φ) "(Hlist & Hcurr_range & Hrange) HΦ".
+      iRevert (curr lvl top_head top L) "Hlist Hcurr_range Hrange HΦ".
+      iLöb as "IH".
+      iIntros (curr lvl top_head top L) "Hlist %Hcurr_range %Hrange HΦ".
+
+      iPoseProof (skip_list_equiv_cons_inv top_head lvl S L top with "Hlist") as "Hlist".
+      iDestruct "Hlist" as (P) "(Hinv & Hlist)".
+
+      wp_lam. wp_let.
+      wp_apply (find_spec with "[Hinv]").
+      { by iFrame. }
+
+      iIntros (pred succ) "(%Hpred_range & %Hpred_key & %Hkey_in_S)".
+      wp_pures. wp_lam. wp_pures.
+      destruct (node_down pred) as [d|] eqn:Hcurr_down; wp_pures.
+      + wp_bind (Load _).
+        destruct L as [|bot].
+        - iDestruct "Hlist" as "(#Hinv & %Hnone & Heq)".
+          iInv (levelN lvl) as (L') "(>%Hperm & >%Hsort & Hlist)" "Hclose".
+
+          destruct Hpred_range as [|Hin]; first by congruence.
+          rewrite -elem_of_elements elem_of_list_In -Hperm in Hin.
+          rewrite list_equiv_invert_L; last done.
+          iDestruct "Hlist" as (? ? ?) "(_ & _ & _ & _ & HP & _)".
+          iMod "HP" as %Hfalse; congruence.
+        - iDestruct "Hlist" as (l down) "(#Hinv & %Hsome & Hpt & %Hmin & Hmatch)".
+          iInv (levelN lvl) as (L') "(>%Hperm & >%Hsort & Hlist)" "Hclose".
+
+          destruct Hpred_range as [Heq|Hin].
+          * assert (d = l) as -> by congruence.
+            wp_load.
+            iMod ("Hclose" with "[Hlist]") as "_".
+            { iNext; iExists L'; by iFrame. }
+
+            iModIntro; wp_let.
+            iApply ("IH" $! down (lvl - 1) down bot L with "[$] [%] [%]").
+            { by left. }
+            { rewrite -Hmin -Heq; lia. }
+            iNext; iIntros (pred' succ') "(Hlist & %Hkey_in_S')".
+            iApply "HΦ"; iSplit; last done. 
+            iExists l, down. by iFrame "# ∗".
+          * rewrite -elem_of_elements elem_of_list_In -Hperm in Hin.
+            rewrite list_equiv_invert_L; last done.
+            iDestruct "Hlist" as (succ' l' γ) "(Hsucc'_range & Hsome' & Hpt' & Hlock & HP & Himp)".
+            iDestruct "HP" as (d' down') "(Hsome_down & Hpt_down & Hin_bot & Hdown'_key)".
+            iMod "Hsome_down" as %Hsome_down; 
+            iMod "Hin_bot" as %Hin_bot; 
+            iMod "Hdown'_key" as %Hdown'_key.
+            
+            assert (d = d') as <- by congruence.
+            iMod "Hpt_down"; wp_load.
+            iMod ("Hclose" with "[Hpt' Hpt_down Himp]") as "_".
+            { 
+              iNext; iExists L'.
+              iPoseProof ("Himp" with "[Hpt' Hpt_down]") as "Hlist".
+              { iFrame; iExists d, down'; by iFrame. }
+              by iFrame.
+            }
+
+            iModIntro; wp_let.
+            iDestruct "Hsucc'_range" as %Hsucc'_range; 
+            iDestruct "Hsome'" as %Hsome'.
+            iApply ("IH" $! down' (lvl - 1) down bot L with "[$] [%] [%]").
+            { by right. }
+            { rewrite -Hdown'_key; lia. }
+            iNext; iIntros (pred'' succ'') "(Hlist & %Hkey_in_S'')".
+            iApply "HΦ"; iSplit; last done.
+            iExists l, down. by iFrame "# ∗".
+      + destruct L as [|bot].
+        - iModIntro. iApply "HΦ".
+          iDestruct "Hlist" as "(#Hinv & %Hnone & %Heq)".
+          rewrite -Heq; by iFrame "#".
+        - iDestruct "Hlist" as (l down) "(#Hinv & %Hsome & Hpt & Hmatch)".
+          iInv (levelN lvl) as (L') "(>%Hperm & >%Hsort & Hlist)" "Hclose".
+
+          destruct Hpred_range as [|Hin]; first by congruence.
+          rewrite -elem_of_elements elem_of_list_In -Hperm in Hin.
+          rewrite list_equiv_invert_L; last done.
+          iDestruct "Hlist" as (? ? ?) "(_ & _ & _ & _ & HP & _)".
+          iDestruct "HP" as (? ?) "(Hfalse & _)".
+          iMod "Hfalse" as %Hfalse; congruence.
+    Qed.
     
     Theorem contains_spec (v: val) (key: Z) (Skeys: gset Z)
       (Hrange: INT_MIN < key < INT_MAX) :
-      {{{ is_skip_list N v Skeys }}}
+      {{{ is_skip_list v Skeys }}}
         contains v #key
       {{{ (b: bool), RET #b; 
-        is_skip_list N v Skeys
+        is_skip_list v Skeys
         ∗
         ⌜ if b then key ∈ Skeys else key ∉ Skeys ⌝
       }}}.
     Proof.
       iIntros (Φ) "H HΦ".
-      iDestruct "H" as (h head S) "(%Hequiv & %Hv & Hpt & %Hmin & #Hinv)".
+      iDestruct "H" as (h head S L) "(%Hequiv & %Hv & Hpt & %Hmin & Hlist)".
       wp_lam. wp_let. rewrite -Hv. wp_load.
-      wp_apply (findPred_spec).
+      wp_apply (findPred_spec with "[Hlist]").
       { iFrame "# ∗". iPureIntro; split. by left. lia. }
-      iIntros (pred succ) "%Hkey_in_S".
+      iIntros (pred succ) "(Hlist & %Hkey_in_S)".
       wp_let. wp_match. wp_pures. wp_lam. wp_pures.
 
       iModIntro; case_bool_decide.
-      + iApply "HΦ". iSplit.
-        - iExists h, head, S. by iFrame "# ∗".
-        - iPureIntro. rewrite /key_equiv in Hequiv. 
-          rewrite -elem_of_elements Hequiv Hkey_in_S.
-          congruence.
       + iApply "HΦ". iSplit. 
-        - iExists h, head, S. by iFrame "# ∗".
-        - iPureIntro. intros Hin. 
-          rewrite -elem_of_elements Hequiv Hkey_in_S in Hin.
-          congruence.
+        iExists h, head, S, L.
+        { by iFrame "# ∗". }
+        iPureIntro. rewrite /key_equiv in Hequiv. 
+        rewrite -elem_of_elements Hequiv Hkey_in_S.
+        congruence.
+      + iApply "HΦ". iSplit. 
+        iExists h, head, S, L.
+        { by iFrame "# ∗". }
+        iPureIntro. intros Hin. 
+        rewrite -elem_of_elements Hequiv Hkey_in_S in Hin.
+        congruence.
     Qed.
 
   End Proofs.
